compiler/dsl/coq/ReflexHVec.v
@@ -1,3 +1,4 @@
+Require Import ReflexBase.
 Require Import ReflexDenoted.
 Require Import ReflexFin.
 Require Import ReflexVec.
@@ -34,11 +35,76 @@ Fixpoint shvec_ith (n : nat) :
     end
   end.
 
+Axiom TODO : forall {T}, T.
+
+Variable desc_eqdec : forall (x y : desc), decide (x = y).
+Variable d : desc.
+Variable x : s[[ d ]].
+
+Fixpoint shvec_in (n : nat) :
+  forall (vd : svec desc n), shvec n vd -> Prop :=
+  match n with
+  | O => fun _ _ => False
+  | S n' => fun vd =>
+    match vd as _vd return shvec (S n') _vd -> Prop with
+    | (dd, vd') => fun vv =>
+      let (v, vv') := vv in
+      match desc_eqdec d dd with
+      | left EQ =>
+        (* need to cast v from s[[ dd ]] into s[[ d ]] to write eq *)
+        match EQ in eq _ _dd return s[[ _dd ]] -> Prop with
+        | eq_refl => fun v => v = x \/ shvec_in n' vd' vv'
+        end v
+      | right N => shvec_in n' vd' vv'
+      end
+    end
+  end.
+
+Variable repr_eqdec : forall (d : desc) (x y : s[[ d ]]), decide (x = y).
+
+Fixpoint shvec_in_dec (n : nat) :
+  forall (vd : svec desc n) (vv : shvec n vd), decide (shvec_in _ vd vv).
+Proof.
+  destruct n.
+  simpl. refine (fun _ _ => right _ _). exact (fun x => match x with end).
+  simpl.
+  intros vd. destruct vd as [dd vd'].
+  intros vv. destruct vv as [v vv'].
+  destruct (desc_eqdec d dd).
+  destruct e.
+  destruct (repr_eqdec _ v x). left; tauto.
+  destruct (shvec_in_dec _ _ vv'). left; tauto.
+  right; tauto.
+  exact (shvec_in_dec _ _ vv').
+Qed.
+
 End SHeterogeneousVector.
 
 Implicit Arguments shvec [desc n].
 
 Implicit Arguments shvec_ith [desc n].
+
+Implicit Arguments shvec_in [desc n].
+
+Theorem shvec_ith_in
+  (desc : Set) (sdenote_desc : desc -> Set) desc_eqdec
+  (UIP_refl_desc : forall (d : desc) (e : d = d), e = Logic.eq_refl d) (n : nat) :
+  forall (vd : svec desc n) v i,
+  shvec_in sdenote_desc desc_eqdec _ (shvec_ith _ vd v i) vd v.
+Proof.
+  intros. induction n. contradiction.
+  simpl in vd. destruct vd as [d vd].
+  simpl in v. destruct v as [x v].
+  simpl in i. destruct i as [i|].
+  simpl. destruct (desc_eqdec (svec_ith vd i) d).
+  subst. right. apply IHn.
+  apply IHn.
+  simpl. destruct (desc_eqdec d d).
+  rewrite (UIP_refl_desc _ e). now left.
+  congruence.
+Qed.
+
+Implicit Arguments shvec_ith_in [desc n].
 
 Section HeterogeneousVector.
 
